### Ejercicio 3

Calcular: $(\frac{(2\frac{3}{5}:3)^{-1}}{(\frac{9}{4})^{2}(\frac{2}{5})^{-1}})$


#### Soluci√≥n

Reescribimos $(2\frac{3}{5}:3)^{-1}$ como:

$\frac{1}{\frac{2\frac{3}{5}}{3}}$

Simplificando:

$= \frac{3}{2 \frac{3}{5}}$


Calculando ${(\frac{9}{4})^{2}(\frac{2}{5})^{-1}}$:


$= \frac{9^2}{4^2} \cdot \frac{1}{\frac{2}{5}}$

$= \frac{81}{16} \cdot \frac{5}{2}$

$= \frac{405}{32}$



Tenemos:

$\frac{\frac{3}{2 \frac{3}{5}}}{\frac{405}{32}}$

Simplificando:

$= \frac{96}{1053}$


$= \frac{32}{351}$

Por tanto:


$(\frac{(2\frac{3}{5}:3)^{-1}}{(\frac{9}{4})^{2}(\frac{2}{5})^{-1}}) = \frac{32}{351}$